high2/Zeta.High.Interleave.fsti
@@ -2,6 +2,9 @@ module Zeta.High.Interleave
 
 open FStar.Seq
 open Zeta.App
+open Zeta.Key
+open Zeta.GenKey
+open Zeta.Record
 open Zeta.Generic.Interleave
 open Zeta.High.Verifier
 open Zeta.EAC
@@ -25,6 +28,10 @@ let gen_seq (app: app_params)
 let verifiable_log (app:_) (n:nat)
   = il:ilog app n {verifiable il}
 
+let thread_store (#app #n:_) (tid: nat{tid < n}) (il: verifiable_log app n)
+  = let vs = thread_state tid il in
+    vs.st
+
 val mk_vlog_entry_ext (#app: app_params) (#n:nat)
   : IF.idxfn_t (gen_seq app n) (vlog_entry_ext app)
 
@@ -42,6 +49,36 @@ let vlog_ext_of_il_log (#app: app_params) (#n:nat)
 val is_eac (#app #n:_) (il: verifiable_log app n)
   : b:bool{b <==> eac (vlog_ext_of_il_log il)}
 
+(* state after processing the i'th element *)
+val eac_state_of_key (#app #n:_) (k: base_key)
+  : IF.seqfn_t (gen_seq app n) (eac_state app k)
+
+(* is the key k in evicted state in *)
+let is_eac_state_evicted (#app #n:_) (k: base_key) (il: verifiable_log app n): bool
+  = EACEvictedMerkle? (eac_state_of_key k il) ||
+    EACEvictedBlum? (eac_state_of_key k il)
+
+val eac_value (#app #n:_) (gk: key app)
+  : IF.seqfn_t (gen_seq app n) (value_t gk)
+
+val empty_implies_eac (#app #n:_) (il: verifiable_log app n)
+  : Lemma (ensures (length il = 0 ==> is_eac il))
+
+val eac_state_transition (#app #n:_) (k: base_key)
+  (il: verifiable_log app n) (i: seq_index il)
+  : Lemma (ensures (let es_pre = IF.to_pre_fn (eac_state_of_key k) il i in
+                    let es_post = IF.to_post_fn (eac_state_of_key k) il i in
+                    let smk = eac_smk app k in
+                    let ee = mk_vlog_entry_ext il i in
+                    es_post = eac_add ee es_pre))
+
+val eac_implies_eac_state_valid (#app #n:_) (k: base_key)
+  (il: verifiable_log app n)
+  : Lemma (ensures (is_eac il ==> eac_state_of_key k il <> EACFail))
+
+val eac_state_of_root_init (#app #n:_) (il: verifiable_log app n)
+  : Lemma (ensures (eac_state_of_key Zeta.BinTree.Root il = EACInit))
+
 let eac_log (app: app_params) (n:nat) = il: verifiable_log app n {is_eac il}
 
 let neac_log (app: app_params) (n:nat) = il: verifiable_log app n {not (is_eac il)}
@@ -54,6 +91,7 @@ val lemma_eac_implies_appfn_calls_seq_consistent (#app #n:_) (il: eac_log app n)
   : Lemma (ensures (let gl = to_glog il in
                     Zeta.AppSimulate.seq_consistent (G.appfn_calls gl)))
 
+
 val eac_boundary (#app #n:_) (il: neac_log app n)
   : (i: seq_index il{is_eac (prefix il i) /\
                      ~ (is_eac (prefix il (i+1)))})
@@ -63,3 +101,4 @@ val eac_boundary_not_appfn (#app #n:_) (il: neac_log app n)
   : Lemma (ensures (let i = eac_boundary il in
                     let e = I.index il i in
                     not (V.is_appfn e)))
+
