high2/Zeta.High.Verifier.EAC.fst
@@ -1,5 +1,7 @@
 module Zeta.High.Verifier.EAC
 
+open Zeta.High.Interleave
+
 module GI=Zeta.Generic.Interleave
 module GTL=Zeta.Generic.TSLog
 module HI=Zeta.High.Interleave
@@ -11,4 +13,5 @@ let lemma_neac_implies_hash_collision
   (itsl: neac_before_epoch app n epmax {GI.aems_equal_upto epmax itsl})
   : hash_collision app
   = let i = HI.eac_boundary itsl in
+    eac_boundary_not_appfn itsl;
     admit()
